Add functions and lemmas

Locally_Nameless_Lambda_Calculus/LN_HO_Term.thy
@@ -3,29 +3,270 @@ theory LN_HO_Term
     Main
     "HOL-Library.Uprod"
     "HOL-Library.Multiset"
+    "HOL-Library.FSet"
+    "HOL-Library.Infinite_Typeclass"
     "HOL-ex.Sketch_and_Explore"
 begin
 
 declare foldl_inject[simp]
 
-datatype (* (plugins del: size) *) (funs_term: 'f, vars_term: 'v) "term" =
+datatype (funs_term: 'f, vars_term: 'v) "term" =
   is_Const: Const 'f |
   is_Free: Free 'v |
   is_Bound: Bound nat |
   is_App: App "('f, 'v) term" "('f, 'v) term" |
   is_Abs: Abs "('f, 'v) term"
 
-(* instantiation "term" :: (type, type) size
-begin
-  primrec size_term :: "('f, 'v) term \<Rightarrow> nat" where
-    "size_term (Const _) = 1" |
-    "size_term (Free _) = 1" |
-    "size_term (Bound _) = 1" |
-    "size_term (App t\<^sub>1 t\<^sub>2) = size_term t\<^sub>1 + size_term t\<^sub>2" |
-    "size_term (Abs t) = 1 + size_term t"
+lemma finite_funs_term: "finite (funs_term t)"
+  by (induction t) simp_all
 
-  instance ..
-end *)
+lemma finite_vars_term: "finite (vars_term t)"
+  by (induction t) simp_all
+
+primrec subst_bound :: "nat \<Rightarrow> ('c, 'f) term \<Rightarrow> ('c, 'f) term \<Rightarrow> ('c, 'f) term" where
+  "subst_bound n t (Const c) = Const c"|
+  "subst_bound n t (Free f) = Free f" |
+  "subst_bound n t (Bound k) = (if k = n then t else Bound k)" |
+  "subst_bound n t (App t\<^sub>1 t\<^sub>2) = App (subst_bound n t t\<^sub>1) (subst_bound n t t\<^sub>2)" |
+  "subst_bound n t (Abs t\<^sub>1) = Abs (subst_bound (Suc n) t t\<^sub>1)"
+
+primrec subst_free :: "'f \<Rightarrow> ('c, 'f) term \<Rightarrow> ('c, 'f) term \<Rightarrow> ('c, 'f) term" where
+  "subst_free x u (Const c) = Const c"|
+  "subst_free x u (Free y) = (if x = y then u else Free y)" |
+  "subst_free x u (Bound k) = Bound k" |
+  "subst_free x u (App t\<^sub>1 t\<^sub>2) = App (subst_free x u t\<^sub>1) (subst_free x u t\<^sub>2)" |
+  "subst_free x u (Abs t) = Abs (subst_free x u t)"
+
+inductive locally_closed :: "('c, 'f) term \<Rightarrow> bool" where
+  Const: "locally_closed (Const c)" |
+  Free: "locally_closed (Free f)" |
+  App: "locally_closed (App t\<^sub>1 t\<^sub>2)"
+    if "locally_closed t\<^sub>1" and "locally_closed t\<^sub>2" |
+  Abs: "locally_closed (Abs t)"
+    if "\<And>x. x |\<notin>| \<X> \<Longrightarrow> locally_closed (subst_bound 0 (Free x) t)"
+
+lemma locally_closed_App_iff: "locally_closed (App t\<^sub>1 t\<^sub>2) \<longleftrightarrow> locally_closed t\<^sub>1 \<and> locally_closed t\<^sub>2"
+  by (auto elim: locally_closed.cases intro: locally_closed.App)
+
+definition body where
+  "body t \<longleftrightarrow> (\<exists>\<X>. \<forall>x. x |\<notin>| \<X> \<longrightarrow> locally_closed (subst_bound 0 (Free x) t))"
+
+lemma locall_closed_Abs_iff_body: "locally_closed (Abs t) \<longleftrightarrow> body t"
+  by (metis Abs LN_HO_Term.term.simps(13,19,25) body_def locally_closed.cases term.sel(6))
+
+lemma subst_bound_subst_bound_Free_idem[simp]:
+  "subst_bound n u (subst_bound n (Free x) t) = subst_bound n (Free x) t"
+  by (induction t arbitrary: n) simp_all
+
+lemma subst_bound_idem_if_subst_bound_subst_bound_idem:
+  "i \<noteq> j \<Longrightarrow>
+  subst_bound i (Free u) (subst_bound j (Free v) t) = subst_bound j (Free v) t \<Longrightarrow>
+  subst_bound i (Free u) t = t"
+proof (induction t arbitrary: i j)
+  case (Bound x)
+  then show ?case
+    by auto
+next
+  case (Abs t)
+  then show ?case
+    unfolding subst_bound.simps term.inject
+    by force
+qed simp_all
+
+lemma subst_bound_idem_if_locally_closed:
+  fixes t :: "('f, 'v) term"
+  assumes inf_vars: "infinite (UNIV :: 'v set)"
+  assumes "locally_closed t"
+  shows "subst_bound n u t = t"
+  using \<open>locally_closed t\<close>
+proof (induction t arbitrary: n u rule: locally_closed.induct)
+  case (Const c)
+  then show ?case by simp
+next
+  case (Free c)
+  then show ?case by simp
+next
+  case (App t\<^sub>1 t\<^sub>2)
+  then show ?case by simp
+next
+  case (Abs \<X> t)
+  obtain x where "x |\<notin>| \<X>"
+    using inf_vars
+    by (metis assms(1) finite_fset ex_new_if_finite)
+
+  then have IH': "\<And>n u. subst_bound n u (subst_bound 0 (Free x) t) = subst_bound 0 (Free x) t"
+    using Abs.IH by auto
+
+  show ?case
+    using subst_bound_idem_if_subst_bound_subst_bound_idem[of _ 0]
+    by (metis IH' nat.distinct(1) subst_bound.simps(5) subst_bound_subst_bound_Free_idem)
+qed
+
+lemma subst_free_term_subst_bound_Free_eq_subst_bound_term:
+  assumes "x \<notin> vars_term t"
+  shows "subst_free x u (subst_bound n (Free x) t) = subst_bound n u t"
+  using assms
+proof (induction t arbitrary: n)
+  case (Const x)
+  then show ?case
+    by simp
+next
+  case (Free y)
+  then have "x \<noteq> y"
+    by simp
+  then show ?case
+    by simp
+next
+  case (Bound i)
+  then show ?case
+    by (auto split: if_split)
+next
+  case (App t1 t2)
+  then show ?case
+    by simp
+next
+  case (Abs t)
+  have "x \<notin> vars_term t"
+    using Abs.prems by simp
+  then have "\<And>n. subst_free x u (subst_bound n (Free x) t) = subst_bound n u t"
+    using Abs.IH by simp
+  then show ?case
+    by simp
+qed
+
+lemma subst_free_commutes_with_subst_bound_Free:
+  fixes t :: "('f, 'v) term"
+  assumes inf_vars: "infinite (UNIV :: 'v set)"
+  assumes "x \<noteq> y" and "locally_closed u"
+  shows "subst_free x u (subst_bound n (Free y) t) = subst_bound n (Free y) (subst_free x u t)"
+proof (induction t arbitrary: n)
+  case (Const x)
+  then show ?case
+    by simp
+next
+  case (Free z)
+  then show ?case
+    unfolding subst_bound.simps
+    by (cases "x = z")
+      (simp_all add: subst_bound_idem_if_locally_closed[OF inf_vars \<open>locally_closed u\<close>])
+next
+  case (Bound i)
+  then show ?case
+    using \<open>x \<noteq> y\<close> by simp
+next
+  case (App t1 t2)
+  then show ?case
+    by simp
+next
+  case (Abs t)
+  then show ?case
+    by simp
+qed
+
+lemma locally_closed_subst_free:
+  fixes t u :: "('f, 'v) term"
+  assumes
+    inf_vars: "infinite (UNIV :: 'v set)" and
+    "locally_closed t" and "locally_closed u"
+  shows "locally_closed (subst_free x u t)"
+  using \<open>locally_closed t\<close>
+proof (induction t rule: locally_closed.induct)
+  case (Const c)
+  then show ?case
+    by (simp add: locally_closed.Const)
+next
+  case (Free f)
+  then show ?case
+    using \<open>locally_closed u\<close>
+    by (simp add: locally_closed.Free)
+next
+  case (App t\<^sub>1 t\<^sub>2)
+  then show ?case
+    by (simp add: locally_closed.App)
+next   
+  case (Abs \<X> t)
+  show ?case
+    unfolding subst_free.simps
+  proof (rule locally_closed.Abs)
+    fix y
+    assume "y |\<notin>| finsert x \<X>"
+    hence "x \<noteq> y" and "y |\<notin>| \<X>"
+      by auto
+    show "locally_closed (subst_bound 0 (Free y) (subst_free x u t))"
+      unfolding subst_free_commutes_with_subst_bound_Free[OF inf_vars \<open>x \<noteq> y\<close> \<open>locally_closed u\<close>,
+          symmetric]
+      using Abs.IH[OF \<open>y |\<notin>| \<X>\<close>] .
+  qed
+qed
+
+lemma body_subst_free:
+  fixes t u :: "('f, 'v) term"
+  assumes
+    inf_vars: "infinite (UNIV :: 'v set)" and
+    "body t" and "locally_closed u"
+  shows "body (subst_free x u t)"
+proof -
+  have "locally_closed (subst_free x u (Abs t))"
+  proof (intro locally_closed_subst_free[OF inf_vars])
+    show "locally_closed (Abs t)"
+      using \<open>body t\<close> by (simp add: locall_closed_Abs_iff_body)
+  next
+    show "locally_closed u"
+      using \<open>locally_closed u\<close> .
+  qed
+
+  then show ?thesis
+    by (simp add: locall_closed_Abs_iff_body)
+qed
+
+lemma body_Abs_if_body:
+  fixes t :: "('f, 'v) term"
+  assumes inf_vars: "infinite (UNIV :: 'v set)"
+  shows "body t \<Longrightarrow> body (Abs t)"
+  unfolding body_def
+  apply (induction t)
+      apply (simp_all add: locally_closed.intros)
+    apply (metis Abs subst_bound.simps(3))
+  using subst_bound_idem_if_locally_closed[OF inf_vars]
+   apply (metis Abs subst_bound.simps(4,5))
+  using subst_bound_idem_if_locally_closed[OF inf_vars]
+  by (metis Abs subst_bound.simps(5))
+
+lemma locally_closed_subst_bound:
+  fixes t u :: "('f, 'v) term"
+  assumes inf_vars: "infinite (UNIV :: 'v set)"
+  assumes "body t" and "locally_closed u"
+  shows "locally_closed (subst_bound 0 u t)"
+proof -
+  obtain \<X> where lc_substb_0_t: "\<And>x. x |\<notin>| \<X> \<Longrightarrow> locally_closed (subst_bound 0 (Free x) t)"
+    using \<open>body t\<close>
+    by (metis body_def)
+
+  obtain x where "x \<notin> vars_term t" and "x \<notin> fset \<X>"
+    by (metis Un_iff ex_new_if_finite finite_Un finite_fset finite_vars_term inf_vars)
+
+  then obtain "subst_free x u (subst_bound 0 (Free x) t) = subst_bound 0 u t"
+    using subst_free_term_subst_bound_Free_eq_subst_bound_term by metis
+
+  moreover have "locally_closed (subst_free x u (subst_bound 0 (Free x) t))"
+  proof (rule locally_closed_subst_free[OF inf_vars])
+    show "locally_closed (subst_bound 0 (Free x) t)"
+      using lc_substb_0_t[OF \<open>x \<notin> fset \<X>\<close>] .
+  next
+    show "locally_closed u"
+      using \<open>locally_closed u\<close> .
+  qed
+
+  ultimately show ?thesis
+    by metis
+qed
+
+primrec shift_bound :: "nat \<Rightarrow> ('c, 'f) term \<Rightarrow> ('c, 'f) term" where
+  "shift_bound n (Const c) = Const c" |
+  "shift_bound n (Free f) = Free f" |
+  "shift_bound n (Bound k) = Bound (if k < n then k else Suc k)" |
+  "shift_bound n (App t\<^sub>1 t\<^sub>2) = App (shift_bound n t\<^sub>1) (shift_bound n t\<^sub>2)" |
+  "shift_bound n (Abs t) = Abs (shift_bound (Suc n) t)"
 
 primrec head where
   "head (Const f) = Const f" |
@@ -40,20 +281,6 @@ primrec subterms where
   "subterms (Bound n) = {#Bound n#}" |
   "subterms (App t\<^sub>1 t\<^sub>2) = add_mset (App t\<^sub>1 t\<^sub>2) (subterms t\<^sub>1 + subterms t\<^sub>2)" |
   "subterms (Abs t) = add_mset (Abs t) (subterms t)"
-
-primrec shift_bound :: "nat \<Rightarrow> ('c, 'f) term \<Rightarrow> ('c, 'f) term" where
-  "shift_bound n (Const c) = Const c" |
-  "shift_bound n (Free f) = Free f" |
-  "shift_bound n (Bound k) = Bound (if k < n then k else Suc k)" |
-  "shift_bound n (App t\<^sub>1 t\<^sub>2) = App (shift_bound n t\<^sub>1) (shift_bound n t\<^sub>2)" |
-  "shift_bound n (Abs t) = Abs (shift_bound (Suc n) t)"
-
-primrec subst_bound :: "nat \<Rightarrow> ('c, 'f) term \<Rightarrow> ('c, 'f) term \<Rightarrow> ('c, 'f) term" where
-  "subst_bound n t (Const c) = Const c"|
-  "subst_bound n t (Free f) = Free f" |
-  "subst_bound n t (Bound k) = (if k = n then t else Bound k)" |
-  "subst_bound n t (App t\<^sub>1 t\<^sub>2) = App (subst_bound n t t\<^sub>1) (subst_bound n t t\<^sub>2)" |
-  "subst_bound n t (Abs t\<^sub>1) = Abs (subst_bound (Suc n) (shift_bound 0 t) t\<^sub>1)"
 
 fun beta_reduce where
   "beta_reduce (App (Abs t\<^sub>1) t\<^sub>2) = subst_bound 0 t\<^sub>2 t\<^sub>1" |
@@ -79,15 +306,29 @@ experiment begin
 lemma "is_hnf (App (Const c\<^sub>1) (Const c\<^sub>2))"
   by simp
 
+lemma "is_hnf (App (App (Const c\<^sub>1) (Const c\<^sub>2)) (Const c\<^sub>3))"
+  by simp
+
+lemma "is_hnf (App (Const c\<^sub>1) (App (Const c\<^sub>2) (Const c\<^sub>3)))"
+  by simp
+
+lemma "\<not> is_hnf (App (Abs (Const c\<^sub>1)) (Const c\<^sub>2))"
+  by simp
+
+lemma "is_hnf (Abs (App (Const c\<^sub>1) (Bound 0)))"
+  by simp
+
+lemma "is_hnf (Abs (Abs (App (App (Const c\<^sub>1) (Bound 1)) (Bound 0))))"
+  by simp
+
 end
  
 lemma "is_hnf t \<Longrightarrow> beta_reduce t = t"
 proof (induction t)
   case (App t1 t2)
   then show ?case
-    by (smt (verit, best) beta_reduce.simps(2,3,4,5,6,7,8)
-        is_hnf.simps(4) is_hnf_App.simps(4,5) term.rel_cases
-        term.rel_eq)
+    by (smt (verit, best) beta_reduce.simps(2,3,4,5,6,7,8) is_hnf.simps(4) is_hnf_App.simps(4,5)
+        term.rel_cases term.rel_eq)
 qed simp_all
 
 end
